thys/POPLmark/POPLmark_2B.thy
@@ -1,0 +1,15 @@
+theory POPLmark_2B
+imports POPLmark_1B
+begin
+
+binder_datatype (FTVars: 'tv, FVars: 'v) trm = Var 'v
+  | Abs x::'v "'tv typ" t::"('tv, 'v) trm" binds x in t
+  | App "('tv, 'v) trm" "('tv, 'v) trm"
+  | TAbs X::'tv "'tv typ" t::"('tv, 'v) trm" binds X in t
+  | TApp "('tv, 'v) trm" "'tv typ"
+
+print_theorems
+
+term Var
+
+end
